crates/sui-framework/packages/sui-system/prelude_extra.bpl
@@ -39,3 +39,55 @@ axiom (forall v: Vec($3_validator_Validator), a: int ::
   then $IsValid'u64'(r) && InRangeVec(v, r) && validator_sui_address( ReadVec(v, r) ) == a &&
        (! exists_validator_in_range_sf(v, 0, r, a))
   else r == -1));
+
+// 1.b. for sum_voting_power_by_address
+
+// public native fun all_addresses_exist_sf(vs: &vector<Validator>, addresses: &vector<address>): bool;
+procedure {:inline 2} $3_validator_set_all_addresses_exist_sf(
+           vs: Vec($3_validator_Validator),
+           addresses: Vec(int)) returns (e: bool) {
+    e := (forall i: int :: InRangeVec(addresses, i) ==> exists_validator_in_range_sf(vs, 0, LenVec(vs), ReadVec(addresses, i)));
+    }
+
+// public native fun sum_voting_power_by_addresses_range_sf(vs: &vector<Validator>, addresses: &vector<address>,
+//     from: u64, to: u64): Integer;
+// ... callable from move
+procedure {:inline 1} $3_validator_set_sum_voting_power_by_addresses_range_sf(
+   vs: Vec($3_validator_Validator),
+   addresses: Vec(int),
+   from: int,
+   to: int) returns (sum: int) {
+   sum := sum_voting_power_by_addresses_range_sf(vs, addresses, from, to);
+   }
+// ... and from Boogie
+function sum_voting_power_by_addresses_range_sf(
+   vs: Vec($3_validator_Validator),
+   addresses: Vec(int),
+   from: int,
+   to: int): int; // defined by axioms
+
+// the sum over an empty range is zero
+axiom (forall vs: Vec($3_validator_Validator), addresses: Vec(int), from: int, to: int ::
+   { sum_voting_power_by_addresses_range_sf(vs, addresses, from, to)}
+   (from >= to ==> sum_voting_power_by_addresses_range_sf(vs, addresses, from, to) == 0));
+
+// the sum of a range can be split in two
+axiom (forall vs: Vec($3_validator_Validator), addresses: Vec(int), a: int, b: int, c: int, d: int ::
+  { sum_voting_power_by_addresses_range_sf(vs, addresses, a, b), sum_voting_power_by_addresses_range_sf(vs, addresses, c, d) }
+  0 <= a && a <= b && b == c && c <= d && d <= LenVec(addresses) ==>
+    sum_voting_power_by_addresses_range_sf(vs, addresses, a, b)
+    + sum_voting_power_by_addresses_range_sf(vs, addresses, c, d)
+    == sum_voting_power_by_addresses_range_sf(vs, addresses, a, d)) ;
+
+// the sum over a singleton range is the vector element there
+axiom (forall vs: Vec($3_validator_Validator), addresses: Vec(int), a: int, x: int, y: int ::
+   { sum_voting_power_by_addresses_range_sf(vs, addresses, x, y),
+     addresses->v[a] }
+    // in a proof involving sum_voting_power_by_addresses_range_sf(vs, addresses,...) and v[a]
+   0 <= a && a + 1 <= LenVec(addresses)  ==> sum_voting_power_by_addresses_range_sf(vs, addresses, a, a+1) ==
+   ReadVec(vs, find_validator_sf(vs, ReadVec(addresses, a)))->$voting_power);
+
+// for vectors of u64, nested ranges have sums bounded by the larger
+axiom (forall vs: Vec($3_validator_Validator), addresses: Vec(int), a: int, b: int, c: int, d: int ::
+  { sum_voting_power_by_addresses_range_sf(vs, addresses, a, d), sum_voting_power_by_addresses_range_sf(vs, addresses, b, c) }
+  $IsValid'vec'$3_validator_Validator''(vs) && 0 <= a && a <= b && b <= c && c <= d && d <= LenVec(addresses)  ==> sum_voting_power_by_addresses_range_sf(vs, addresses, b, c) <= sum_voting_power_by_addresses_range_sf(vs, addresses, a, d)) ;
